WIP on typing fixBy as generated by the compiler

examples/recursion/src/Lib.hs
@@ -1,0 +1,26 @@
+--
+-- Necessary language extensions for the Plutus Tx compiler to work.
+{-# LANGUAGE DataKinds           #-}
+{-# LANGUAGE NoImplicitPrelude   #-}
+{-# LANGUAGE ScopedTypeVariables #-}
+{-# LANGUAGE TemplateHaskell     #-}
+module Lib where
+
+import qualified Language.PlutusCore.Builtins as PLC
+import qualified Language.PlutusCore.Universe as PLC
+-- Main Plutus Tx module.
+import           Language.PlutusTx
+-- Additional support for lifting.
+import           Language.PlutusTx.Lift
+-- Builtin functions.
+import           Language.PlutusTx.Builtins
+-- The Plutus Tx Prelude, discussed further below.
+import           Language.PlutusTx.Prelude
+
+pastEnd :: CompiledCode (Integer -> Bool)
+pastEnd = $$(compile [|| \(y :: Integer) ->
+    let
+        z = addInteger y w
+        w = addInteger y z
+    in lessThanEqInteger z w
+  ||])
